extraction/theories/ErasureCorrectness.v
@@ -11,6 +11,7 @@ From Coq Require Import String.
 From Equations Require Import Equations.
 From MetaCoq.Erasure Require Import ErasureCorrectness.
 From MetaCoq.Erasure Require Import ErasureFunction.
+From MetaCoq.Erasure Require Import ESubstitution.
 From MetaCoq.Erasure Require Import EWcbvEval.
 From MetaCoq.Erasure Require Import Extract.
 From MetaCoq.PCUIC Require Import PCUICAstUtils.
@@ -18,6 +19,7 @@ From MetaCoq.PCUIC Require Import PCUICInduction.
 From MetaCoq.PCUIC Require Import PCUICSafeLemmata.
 From MetaCoq.PCUIC Require Import PCUICTyping.
 From MetaCoq.PCUIC Require Import PCUICWcbvEval.
+From MetaCoq.PCUIC Require Import PCUICWeakeningEnv.
 From MetaCoq.Template Require Import BasicAst.
 From MetaCoq.Template Require Import utils.
 
@@ -30,6 +32,132 @@ Module E := EAst.
 
 Notation "Σ 'p⊢' s ▷ t" := (PCUICWcbvEval.eval Σ s t) (at level 50, s, t at next level) : type_scope.
 Notation "Σ 'e⊢' s ▷ t" := (EWcbvEval.eval Σ s t) (at level 50, s, t at next level) : type_scope.
+
+Lemma contains_In k ks :
+  Erasure.contains k ks <-> In k ks.
+Proof.
+  split; intros.
+  - unfold contains in *.
+    apply existsb_exists in H as (? & ? & ?).
+    unfold eq_kername in *.
+    now destruct kername_eq_dec as [<-|].
+  - unfold contains.
+    induction ks; cbn in *; [easy|].
+    destruct H as [->|].
+    + now rewrite eq_kername_refl.
+    + rewrite IHks by easy.
+      now rewrite Bool.orb_true_r.
+Qed.
+
+Lemma erases_deps_forall_ind Σ Σ'
+  (P : Extract.E.term -> Prop)
+  (Hbox : P Extract.E.tBox)
+  (Hrel : forall i : nat, P (Extract.E.tRel i))
+  (Hvar : forall n : ident, P (Extract.E.tVar n))
+  (Hevar :
+     forall (m : nat) (l : list Extract.E.term),
+       Forall P l ->
+       Forall (erases_deps Σ Σ') l -> P (Extract.E.tEvar m l))
+  (Hlam : forall (na : name) (body : Extract.E.term),
+        erases_deps Σ Σ' body -> P body -> P (Extract.E.tLambda na body))
+  (Hletin : forall (na : name) (val body : Extract.E.term),
+        erases_deps Σ Σ' val ->
+        P val -> erases_deps Σ Σ' body -> P body -> P (Extract.E.tLetIn na val body))
+  (Happ : forall hd arg : Extract.E.term,
+        erases_deps Σ Σ' hd -> P hd -> erases_deps Σ Σ' arg -> P arg -> P (Extract.E.tApp hd arg))
+  (Hconst : forall (kn : kername) (n : nat) (cb : MetaCoqErasureCorrectnessStrong.PA.constant_body)
+                   (Σsuf : list (kername × MetaCoqErasureCorrectnessStrong.PA.global_decl))
+                   (cb' : EAst.constant_body),
+      skipn n Σ = (kn, MetaCoqErasureCorrectnessStrong.PA.ConstantDecl cb) :: Σsuf ->
+      ETyping.declared_constant Σ' kn cb' ->
+      erases_constant_body (Σsuf, PCUICAst.cst_universes cb) cb cb' ->
+      (forall body : Extract.E.term, Extract.E.cst_body cb' = Some body -> erases_deps Σ Σ' body) ->
+      (forall body : Extract.E.term, Extract.E.cst_body cb' = Some body -> P body) ->
+ P (Extract.E.tConst kn))
+  (Hconstruct : forall (ind : inductive) (c : nat), P (Extract.E.tConstruct ind c))
+  (Hcase : forall (p : inductive × nat) (discr : Extract.E.term) (brs : list (nat × Extract.E.term)),
+        erases_deps Σ Σ' discr ->
+        P discr ->
+        Forall (fun br : nat × Extract.E.term => erases_deps Σ Σ' br.2) brs ->
+        Forall (fun br => P br.2) brs ->
+        P (Extract.E.tCase p discr brs))
+  (Hproj : forall (p : projection) (t : Extract.E.term),
+        erases_deps Σ Σ' t -> P t -> P (Extract.E.tProj p t))
+  (Hfix : forall (defs : list (Extract.E.def Extract.E.term)) (i : nat),
+         Forall (fun d : Extract.E.def Extract.E.term => erases_deps Σ Σ' (Extract.E.dbody d)) defs ->
+         Forall (fun d => P (E.dbody d)) defs ->
+         P (Extract.E.tFix defs i))
+  (Hcofix : forall (defs : list (Extract.E.def Extract.E.term)) (i : nat),
+         Forall (fun d : Extract.E.def Extract.E.term => erases_deps Σ Σ' (Extract.E.dbody d)) defs ->
+         Forall (fun d => P (E.dbody d)) defs ->
+         P (Extract.E.tCoFix defs i)) :
+  forall t, erases_deps Σ Σ' t -> P t.
+Proof.
+  fix f 2.
+  intros t ed.
+  move f at top.
+  destruct ed;
+    try solve [match goal with
+    | [H: _ |- _] => apply H
+    end; auto].
+  - apply Hevar; [|assumption].
+    revert l H.
+    fix f' 2.
+    intros l [].
+    + now constructor.
+    + constructor; [now apply f|now apply f'].
+  - eapply Hconst; try eassumption.
+    intros.
+    apply f.
+    now apply H2.
+  - apply Hcase; try assumption.
+    + now apply f.
+    + revert brs H.
+      fix f' 2.
+      intros brs []; [now constructor|].
+      constructor; [now apply f|now apply f'].
+  - apply Hfix; try assumption.
+    revert defs H.
+    fix f' 2.
+    intros defs []; [now constructor|].
+    constructor; [now apply f|now apply f'].
+  - apply Hcofix; try assumption.
+    revert defs H.
+    fix f' 2.
+    intros defs []; [now constructor|].
+    constructor; [now apply f|now apply f'].
+Defined.
+
+Lemma erases_deps_cons Σ Σ' kn decl t :
+  fresh_global kn Σ ->
+  erases_deps Σ Σ' t ->
+  erases_deps ((kn, decl) :: Σ) Σ' t.
+Proof.
+  intros fresh er.
+  induction er using erases_deps_forall_ind; try solve [now constructor].
+  econstructor.
+  - rewrite skipn_S.
+    eassumption.
+    (*unfold declared_constant.
+    cbn.
+    unfold eq_kername.
+    destruct kername_eq_dec as [<-|]; [congruence|].
+    eassumption.*)
+  - eassumption.
+  - eassumption.
+  - easy.
+  (*- unfold erases_constant_body in *.
+    destruct PCUICAst.cst_body eqn:body.
+    + destruct E.cst_body eqn:ebody; [|easy].
+      pose proof erases_extends.
+      red in X.
+      inversion wfΣ; subst.
+      specialize (X (Σ, PCUICAst.cst_universes cb) ltac:(easy) [] t).
+      clear -H0 fresh.
+k      admit.
+    + now destruct E.cst_body.
+  - easy.*)
+Qed.
 
 Lemma erase_global_decls_deps_recursive_correct Σ wfΣ include ignore erase_func Σex :
   (forall k, ignore k = false) ->
@@ -59,8 +187,36 @@ Ltac unproof :=
     end.
 
   intros no_ignores er.
-  induction Σ as [|(kn, decl) Σ IH] in wfΣ, include, Σex, er |- *; intros k isin;
-    [easy|].
+  induction Σ as [|(kn, decl) Σ IH] in wfΣ, include, Σex, er |- *; [easy|].
+  cbn in *; unproof.
+  rewrite no_ignores in er.
+  destruct (contains kn include) eqn:contains; cycle 1.
+  - cbn in *.
+    intros.
+    eapply IH with (k := k) in er; eauto.
+    unfold eq_kername.
+    destruct kername_eq_dec as [->|].
+    + now apply contains_In in H.
+    + destruct P.lookup_env; [|easy].
+      destruct g; [|easy].
+      destruct wfΣ.
+      inversion X; subst; clear X.
+      now apply erases_deps_cons.
+  - cbn in *.
+    destruct erase_global_decl eqn:erdecl; cbn in *; [|congruence].
+    destruct erase_global_decls_deps_recursive eqn:errec; [|congruence].
+    inversion er; subst; clear er.
+    eapply IH in errec.
+  - cbn in *.
+    destruct erase_global_decl eqn:erdecl; [|congruence].
+    inversion er; subst; clear er.
+    cbn in *.
+    destruct decl; cycle 1.
+    * simpl in erdecl.
+  rew
+  destruct P.lookup_env eqn:lookup; [|easy].
+  destruct g; [|easy].
+  cbn in *; unproof.
   Admitted.
 (*  cbn.
   cbn in *; unproof.
